CoqOfRust/core/convert/links/mod.v
@@ -2,8 +2,6 @@ Require Import CoqOfRust.CoqOfRust.
 Require Import links.M.
 Require Import core.convert.mod.
 
-Import Run.
-
 (*
 pub trait From<T>: Sized {
     fn from(value: T) -> Self;
@@ -19,7 +17,7 @@ Module From.
       Run.Trait method [] [] [ φ value ] Self
     ).
 
-  Record Run (Self : Set) {T : Set} `{Link Self} `{Link T} : Set := {
+  Class Run (Self : Set) {T : Set} `{Link Self} `{Link T} : Set := {
     from : Run_from Self T;
   }.
 End From.
